src/proof/kubernetes_model/create_named_orphan.v
@@ -1,0 +1,510 @@
+From New.proof Require Import prelude empty_ffi.
+From New.proof.kubernetes_model Require Export create_named.
+
+Section proof.
+Context `{hG: !heapGS Σ} `{!ffi_semantics _ _}.
+Context {sem : go.Semantics} {package_sem : apimodel.Assumptions}.
+Context `{!kubernetesModelG Σ}.
+Local Set Default Proof Using "All".
+
+Lemma wp_State__create_named_orphan_au γ l kind namespace key i kobj :
+  ∀ Φ,
+  ( is_pkg_init apimodel ∗
+    is_kubernetes γ l ∗
+    "%Hvalid" ∷ ⌜ KObjectV.valid_named_create kind namespace kobj ⌝ ∗
+    "%Hns_nonempty" ∷ ⌜ namespace ≠ ""%go ⌝ ∗
+    "%Hns_valid" ∷ ⌜ valid_namespace namespace ⌝ ∗
+    "%Hkey_eq" ∷ ⌜ key = {|
+      KKey.Kind' := kind;
+      KKey.Name' := (KObjectV.objectmeta kobj).(ObjectMetaV.Name');
+      KKey.Namespace' := namespace
+    |} ⌝ ∗
+    "%Hparent_none" ∷ ⌜ obj_parent_ref kobj = None ⌝ ∗
+    "Hdeepown_i" ∷ KObjectV.deepown_i i kobj 1 ∗
+    "Hown_reserved_frag" ∷ own_reserved_frag γ key ∗
+    |={⊤,∅}=>
+      "Hclose" ∷ (∀ i' kobj' uid,
+        ⌜ KObjectV.valid kobj' ⌝ ∗
+        ⌜ KObjectV.same_kind kobj kobj' ⌝ ∗
+        ⌜ ObjectMetaV.named_created namespace
+            (KObjectV.objectmeta kobj) (KObjectV.objectmeta kobj') ⌝ ∗
+        ⌜ ObjectSpecV.created
+            (KObjectV.spec kobj) (KObjectV.spec kobj') ⌝ ∗
+        ⌜ ObjectStatusV.created
+            (KObjectV.status kobj) (KObjectV.status kobj') ⌝ ∗
+        ⌜ key = KObjectV.key kobj' ⌝ ∗
+        ⌜ uid = (KObjectV.objectmeta kobj').(ObjectMetaV.UID') ⌝ ∗
+        KObjectV.deepown_i i' kobj' 1 ∗
+        own_meta_frag γ key uid 1 (KObjectV.objectmeta kobj') ∗
+        own_spec_frag γ key uid 1 (KObjectV.spec kobj') ∗
+        own_status_frag γ key uid 1 (KObjectV.status kobj') ∗
+        own_children_frag γ key uid 1 ∅
+          ={∅,⊤}=∗ ▷ Φ (#(interface.ok i'), #interface.nil)%V)
+  ) -∗
+  WP l @! (go.PointerType apimodel.State) @!
+    "create" #kind #namespace #(interface.ok i) {{ Φ }}.
+Proof.
+  iIntros (Φ) "(#Hpkg & #Hkinv & Hau)".
+  iNamed "Hau". iNamed "Hkinv".
+  wp_method_call. rewrite /apimodel.State__createⁱᵐᵖˡ. wp_call.
+  wp_apply wp_with_defer as "%defer Hdefer".
+  simpl subst. wp_auto.
+  wp_apply wp_Mutex__Lock; [done|].
+  iIntros "[Hown_Mutex H]". iNamedPrefix "H" "Hinv_". wp_auto.
+  wp_apply (wp_deepCopy i kobj with "[Hdeepown_i]").
+  { iFrame "#". iExact "Hdeepown_i". }
+  iIntros (i1) "[Hdeepown_i1 Hdeepown_i]". wp_auto.
+  iDestruct "Hdeepown_i1" as (l1) "[%Hvalid_interface Hdeepown_l]".
+  wp_apply wp_Accessor. 1: iPureIntro; done.
+  iPoseProof (KObjectV.deepown_l_split with "Hdeepown_l") as
+    "(%Hl1_not_null & Hdeepown_t_l & Hdeepown_m_l &
+      Hdeepown_s_l & Hdeepown_st_l)".
+  wp_apply (wp_WipeObjectMetaSystemFields with "[$Hdeepown_m_l]").
+  1: done.
+  iIntros (time) "Hdeepown_m_l". wp_auto.
+  wp_apply (wp_EnsureObjectNamespaceMatchesRequestNamespace
+    with "[$Hdeepown_m_l]").
+  { iPureIntro.
+    destruct Hvalid as (_ & _ & Hmeta & _).
+    destruct Hmeta as (_ & _ & _ & Hns & _).
+    destruct Hns as [Hns|(_ & Hns)]; rewrite Hns; auto. }
+  iIntros "Hdeepown_m_l". wp_auto.
+  wp_apply v1.wp_Now.
+  iIntros (now_time now_timev) "Hdeepown_time". wp_auto.
+  wp_apply (wp_SetCreationTimestamp_deepown
+    with "[$Hdeepown_m_l $Hdeepown_time]").
+  iIntros "Hdeepown_m_l". wp_auto.
+  wp_apply (wp_State__generateNewUIDAndUpdate
+    with "[$Hinv_Hstate_used_uid_addr $Hinv_Hown_used_uid]").
+  iIntros (generated_uid)
+    "(%Hgenerated_uid_is_not_used & %Hgenerated_uid_valid &
+      Hinv_Hstate_used_uid_addr & Hinv_Hown_used_uid)".
+  wp_auto.
+  wp_apply (wp_SetUID_deepown with "[$Hdeepown_m_l]").
+  iIntros "Hdeepown_m_l". wp_auto.
+  wp_apply (wp_GetName_deepown with "[$Hdeepown_m_l]").
+  iIntros "Hdeepown_m_l". wp_auto.
+  wp_apply (wp_GetGenerateName_deepown with "[$Hdeepown_m_l]").
+  iIntros "Hdeepown_m_l". wp_auto.
+  assert ((KObjectV.objectmeta kobj).(ObjectMetaV.Name') ≠ ""%go)
+    as Hname_nonempty.
+  { destruct Hvalid as (_ & _ & Hmeta & _).
+    destruct Hmeta as (_ & Hname_nonempty & _).
+    done. }
+  rewrite bool_decide_false //. wp_auto.
+  iPoseProof (KObjectV.deepown_l_merge _ _ _ _ Hl1_not_null
+    with "[$Hdeepown_t_l $Hdeepown_m_l $Hdeepown_s_l $Hdeepown_st_l]")
+    as "Hdeepown_l".
+  wp_apply (wp_applyValidationAndDefaulting with "[Hdeepown_l]").
+  { iFrame.
+    iPureIntro.
+    destruct Hvalid as
+      (Hkind & Hvalid_create_typemeta & Hmeta & _).
+    destruct Hmeta as
+      (Hgn_valid & Hname_nonempty' & Hname_valid & _ &
+       Hlabels & Hannotations & Howner_refs & Hfinalizers &
+       Hmanaged_fields).
+    split.
+    - destruct kobj; done.
+    - split.
+      + rewrite KObjectV.kind_update_objectmeta
+          KObjectV.typemeta_update_objectmeta.
+        exact Hvalid_create_typemeta.
+      + destruct kobj; simpl in Hkind |- *; subst kind;
+          split_and!; done. }
+  iIntros (kobj1)
+    "(Hdeepown_l & %Hsame_kind & %Hvalid_meta & %Hvalid_spec &
+      %Hvalid_status & %Hvalid_typemeta & %Hm_eq &
+      %Hcreated_spec & %Hcreated_status)".
+  wp_auto.
+  iPoseProof (KObjectV.deepown_l_split with "Hdeepown_l") as
+    "(%Hl1_not_null1 & Hdeepown_t_l & Hdeepown_m_l &
+      Hdeepown_s_l & Hdeepown_st_l)".
+  assert (KObjectV.objectmeta_ptr l1 kobj =
+      KObjectV.objectmeta_ptr l1 kobj1) as ->.
+  { destruct kobj, kobj1; done. }
+  assert (KObjectV.kind kobj1 = kind) as Hkind1.
+  { destruct Hvalid as (Hkind & _).
+    destruct kobj, kobj1; simpl in *; subst; done. }
+  wp_apply (wp_validateObjectMeta with "[$Hdeepown_m_l]").
+  { iSplit; first done.
+    iPureIntro. rewrite -Hkind1. exact Hvalid_meta. }
+  iIntros "Hdeepown_m_l". wp_auto.
+  iAssert (⌜ dom phys_state = dom abs_state ⌝%I) as "%Hdom_eq".
+  { iDestruct (big_sepM2_dom with "Hinv_Hphys_abs_rep") as %Hdom_eq.
+    iPureIntro. done. }
+  iPoseProof (reserved_keys.frag_elem_of_auth key
+    with "[$Hinv_Hown_reserved] [$Hown_reserved_frag]")
+    as "%Hkey_reserved".
+  assert (Hkey_not_in_abs : abs_state !! key = None).
+  { apply not_elem_of_dom.
+    Timeout 10 set_solver. }
+  assert (Hkey_not_in_phys : phys_state !! key = None).
+  { apply not_elem_of_dom.
+    apply not_elem_of_dom in Hkey_not_in_abs.
+    rewrite Hdom_eq.
+    done. }
+  wp_apply (wp_map_lookup2 apimodel.KKey (go.InterfaceType [])
+    with "[$Hinv_Hown_phys]").
+  iIntros "Hinv_Hown_phys". wp_auto.
+  rewrite /is_Some.
+  rewrite <- Hkey_eq.
+  rewrite Hkey_not_in_phys.
+  wp_auto.
+  wp_apply (wp_State__generateNewRVAndUpdate
+    with "[$Hinv_Hstate_used_rv_addr $Hinv_Hown_used_rv]").
+  iIntros (generated_rv)
+    "(%Hgenerated_rv_is_not_used & %Hgenerated_rv_valid &
+      Hinv_Hstate_used_rv_addr & Hinv_Hown_used_rv)".
+  wp_auto.
+  wp_apply (wp_SetResourceVersion_deepown with "[$Hdeepown_m_l]").
+  iIntros "Hdeepown_m_l". wp_auto.
+  wp_apply (wp_map_insert apimodel.KKey with "[$Hinv_Hown_phys]").
+  iIntros "Hinv_Hown_phys". wp_auto.
+  iPoseProof (KObjectV.deepown_l_merge _ _ _ _ Hl1_not_null1
+    with "[$Hdeepown_t_l $Hdeepown_m_l $Hdeepown_s_l $Hdeepown_st_l]")
+    as "Hdeepown_l".
+  iAssert (KObjectV.deepown_i i1
+    (KObjectV.update_objectmeta kobj1
+      ((KObjectV.objectmeta kobj1)
+        <| ObjectMetaV.ResourceVersion' := generated_rv |>)) 1)
+    with "[Hdeepown_l]" as "Hdeepown_i1".
+  { iExists l1. iSplit.
+    { iPureIntro. destruct kobj, kobj1. all: done. }
+    iFrame. }
+  wp_apply (wp_deepCopy with "[$Hpkg $Hdeepown_i1]").
+  iIntros (i2) "[Hdeepown_i2 Hdeepown_i1]". wp_auto.
+  set kobj2 := KObjectV.update_objectmeta kobj1
+    ((KObjectV.objectmeta kobj1)
+      <| ObjectMetaV.ResourceVersion' := generated_rv |>).
+  iApply fupd_wp.
+  iMod "Hau" as "Hclose".
+  assert (KObjectV.valid kobj2) as Hvalid2.
+  { subst kobj2.
+    destruct Hvalid as (Hkind_eq & _).
+    destruct kobj; destruct kobj1; try done.
+    all: solve_update_objectmeta_valid
+      Hvalid_typemeta Hgenerated_rv_valid Hvalid_meta
+      Hvalid_spec Hvalid_status. }
+  assert (Hparent_none2 : obj_parent_ref kobj2 = None).
+  { unfold obj_parent_ref in Hparent_none |- *.
+    subst kobj2.
+    rewrite objectmeta_update_objectmeta Hm_eq objectmeta_update_objectmeta.
+    unfold meta_parent_ref in Hparent_none |- *.
+    simpl.
+    destruct
+      ((KObjectV.objectmeta kobj).(ObjectMetaV.OwnerReferences'))
+      as [orefs|] eqn:Horefs; simpl in Hparent_none |- *; [|done].
+    destruct
+      (list_find
+        (λ oref : OwnerReferenceV.t,
+          oref.(OwnerReferenceV.Controller') = Some true)
+        orefs)
+      as [[idx oref]|] eqn:Hfind;
+      simpl in Hparent_none |- *; done. }
+  iPoseProof (kview.own_auth_valid_forall with "[$Hinv_Hown_abs]")
+    as "%Habs_state_valid".
+  iMod (kview.create_kobj_vs key generated_uid kobj2
+    with "[$Hinv_Hown_abs]")
+    as "(Hinv_Hown_abs & Hown_meta & Hown_spec & Hown_status)".
+  { exact Hkey_not_in_abs. }
+  { rewrite Hinv_Hused_uid_eq_dom_phys_used_uid.
+    apply not_elem_of_dom. done. }
+  { unfold kview.valid_k_uid_obj.
+    rewrite Hkey_eq.
+    subst kobj2.
+    split_and!.
+    - destruct Hvalid as (Hkind_eq & _).
+      destruct kobj; destruct kobj1; try done;
+        rewrite Hm_eq; simpl; rewrite Hkind_eq; done.
+    - destruct kobj; destruct kobj1; try done;
+        rewrite Hm_eq; done.
+    - done. }
+  { intros kind' name' uid' Hparent.
+    unfold obj_parent_ref, meta_parent_ref_is in Hparent_none2, Hparent.
+    rewrite Hparent_none2 in Hparent.
+    done. }
+  iMod (cview.create_orphan_vs2 key generated_uid kobj2
+    with "[$Hinv_Hown_children]")
+    as "(Hinv_Hown_children & Hown_children)".
+  { subst kobj2.
+    destruct kobj; destruct kobj1;
+      try done; rewrite Hm_eq; done. }
+  { exact Hkey_not_in_abs. }
+  { exact Hparent_none2. }
+  { rewrite map_Forall_lookup.
+    intros k' obj Hlookup.
+    pose proof (Habs_state_valid _ _ Hlookup)
+      as (_ & _ & _ & Hno_spec & _).
+    rewrite Hinv_Hused_uid_eq_set_map_used_reference in Hno_spec.
+    exact Hno_spec. }
+  { intros Hin.
+    assert (Huid_fresh : generated_uid ∉ used_uid).
+    { apply not_elem_of_dom in Hgenerated_uid_is_not_used.
+      rewrite <- Hinv_Hused_uid_eq_dom_phys_used_uid
+        in Hgenerated_uid_is_not_used.
+      done. }
+    apply Huid_fresh.
+    rewrite Hinv_Hused_uid_eq_set_map_used_reference.
+    done. }
+  iMod (reserved_keys.consume_reserved_key_vs key
+    with "[$Hinv_Hown_reserved] [$Hown_reserved_frag]")
+    as "Hinv_Hown_reserved".
+  iMod ("Hclose" $! i2 kobj2 generated_uid
+    with "[$Hdeepown_i2 $Hown_meta $Hown_spec $Hown_status
+      $Hown_children]") as "HΦ".
+  { iPureIntro. split_and!.
+    - done.
+    - subst kobj2.
+      destruct kobj; destruct kobj1; done.
+    - unfold ObjectMetaV.named_created.
+      subst kobj2.
+      destruct kobj; destruct kobj1;
+        simpl in Hm_eq |- *;
+        try done; rewrite Hm_eq; split_and!; done.
+    - subst kobj2.
+      rewrite KObjectV.spec_update_objectmeta.
+      rewrite KObjectV.spec_update_objectmeta in Hcreated_spec.
+      done.
+    - subst kobj2.
+      rewrite KObjectV.status_update_objectmeta.
+      rewrite KObjectV.status_update_objectmeta in Hcreated_status.
+      done.
+    - subst kobj2.
+      rewrite Hkey_eq.
+      destruct Hvalid as (Hkind_eq & _).
+      destruct kobj; destruct kobj1;
+        simpl in Hsame_kind, Hm_eq, Hkind_eq |- *;
+        try done; rewrite Hm_eq; rewrite Hkind_eq; done.
+    - subst kobj2.
+      destruct kobj; destruct kobj1;
+        simpl in Hm_eq |- *;
+        try done; rewrite Hm_eq; done. }
+  assert (Htombed_uid_new :
+    tombed_uid =
+    (used_uid ∪ {[generated_uid]}) ∖
+      map_to_set
+        (λ _ obj, (KObjectV.objectmeta obj).(ObjectMetaV.UID'))
+        (<[key := kobj2]> abs_state)).
+  { assert (Hobj_uid :
+      generated_uid =
+        (KObjectV.objectmeta kobj2).(ObjectMetaV.UID')).
+    { subst kobj2.
+      destruct kobj; destruct kobj1;
+        simpl in Hm_eq |- *;
+        try done; rewrite Hm_eq; done. }
+    assert (Huid_fresh : generated_uid ∉ used_uid).
+    { apply not_elem_of_dom in Hgenerated_uid_is_not_used.
+      rewrite <- Hinv_Hused_uid_eq_dom_phys_used_uid
+        in Hgenerated_uid_is_not_used.
+      done. }
+    rewrite (map_to_set_insert_L
+      (λ _ obj, (KObjectV.objectmeta obj).(ObjectMetaV.UID'))
+      abs_state key kobj2 Hkey_not_in_abs).
+    rewrite <- Hobj_uid.
+    exact (tombed_uid_create_eq_used_uid_sub
+      used_uid tombed_uid
+      (map_to_set
+        (λ _ obj, (KObjectV.objectmeta obj).(ObjectMetaV.UID'))
+        abs_state)
+      generated_uid Huid_fresh
+      Hinv_Htombed_uid_eq_used_uid_sub). }
+  iModIntro.
+  iAssert (([∗ map] i; obj ∈
+      <[key:=interface.ok i1]> phys_state;
+      <[key:=kobj2]> abs_state,
+    match i with
+    | interface.ok i_ok => KObjectV.deepown_i i_ok obj 1
+    | interface.nil => False%I
+    end)%I)
+    with "[Hdeepown_i1 Hinv_Hphys_abs_rep]"
+    as "Hinv_Hphys_abs_rep".
+  { rewrite (big_sepM2_insert _ phys_state abs_state key
+      (interface.ok i1) kobj2 Hkey_not_in_phys Hkey_not_in_abs).
+    iSplitL "Hdeepown_i1".
+    - iExact "Hdeepown_i1".
+    - iExact "Hinv_Hphys_abs_rep". }
+  iCombineNamed "Hinv_*" as "H".
+  wp_apply (wp_Mutex__Unlock _ (kubernetes_inv γ l)
+    with "[$Hown_Mutex H]").
+  { iNamed "H". iFrame. iFrame "#". iPureIntro. split_and!.
+    - rewrite dom_insert_L.
+      rewrite Hinv_Hused_uid_eq_dom_phys_used_uid.
+      rewrite union_comm_L.
+      done.
+    - assert (Hobj_ref :
+        obj_ref key kobj2 = (key, generated_uid)).
+      { unfold obj_ref.
+        subst kobj2.
+        rewrite Hkey_eq.
+        destruct kobj; destruct kobj1;
+          simpl in Hsame_kind, Hm_eq |- *;
+          try done; rewrite Hm_eq; reflexivity. }
+      assert (Hobj_uid :
+          generated_uid = snd (obj_ref key kobj2)).
+      { rewrite Hobj_ref. done. }
+      rewrite set_map_union_L set_map_singleton_L.
+      rewrite Hinv_Hused_uid_eq_set_map_used_reference.
+      rewrite Hobj_uid.
+      done.
+    - exact Htombed_uid_new.
+    - rewrite dom_insert_L.
+      Timeout 10 set_solver. }
+  iApply "HΦ".
+Unshelve. all: try tc_solve. all: try apply _. all: try exact sem.
+all: try done.
+Qed.
+
+Lemma wp_State__create_named_orphan γ l kind namespace key i kobj :
+  {{{ is_pkg_init apimodel ∗
+      "#Hisk" ∷ is_kubernetes γ l ∗
+      "%Hvalid" ∷
+        ⌜ KObjectV.valid_named_create kind namespace kobj ⌝ ∗
+      "%Hns_nonempty" ∷ ⌜ namespace ≠ ""%go ⌝ ∗
+      "%Hns_valid" ∷ ⌜ valid_namespace namespace ⌝ ∗
+      "%Hkey_eq" ∷ ⌜ key = {|
+        KKey.Kind' := kind;
+        KKey.Name' := (KObjectV.objectmeta kobj).(ObjectMetaV.Name');
+        KKey.Namespace' := namespace
+      |} ⌝ ∗
+      "%Hparent_none" ∷ ⌜ obj_parent_ref kobj = None ⌝ ∗
+      "Hdeepown_i" ∷ KObjectV.deepown_i i kobj 1 ∗
+      "Hown_reserved_frag" ∷ own_reserved_frag γ key
+  }}}
+    l @! (go.PointerType apimodel.State) @!
+      "create" #kind #namespace #(interface.ok i)
+  {{{ i' kobj' uid, RET (#(interface.ok i'), #interface.nil);
+      "%Hvalid'" ∷ ⌜ KObjectV.valid kobj' ⌝ ∗
+      "%Hsame_kind" ∷ ⌜ KObjectV.same_kind kobj kobj' ⌝ ∗
+      "%Hmeta_created" ∷
+        ⌜ ObjectMetaV.named_created namespace
+            (KObjectV.objectmeta kobj) (KObjectV.objectmeta kobj') ⌝ ∗
+      "%Hspec_created" ∷
+        ⌜ ObjectSpecV.created
+            (KObjectV.spec kobj) (KObjectV.spec kobj') ⌝ ∗
+      "%Hstatus_created" ∷
+        ⌜ ObjectStatusV.created
+            (KObjectV.status kobj) (KObjectV.status kobj') ⌝ ∗
+      "%Hkey_eq'" ∷ ⌜ key = KObjectV.key kobj' ⌝ ∗
+      "%Huid_eq" ∷
+        ⌜ uid = (KObjectV.objectmeta kobj').(ObjectMetaV.UID') ⌝ ∗
+      "Hdeepown_i" ∷ KObjectV.deepown_i i' kobj' 1 ∗
+      "Hown_meta_frag" ∷
+        own_meta_frag γ key uid 1 (KObjectV.objectmeta kobj') ∗
+      "Hown_spec_frag" ∷
+        own_spec_frag γ key uid 1 (KObjectV.spec kobj') ∗
+      "Hown_status_frag" ∷
+        own_status_frag γ key uid 1 (KObjectV.status kobj') ∗
+      "Hown_children_frag" ∷ own_children_frag γ key uid 1 ∅
+  }}}.
+Proof.
+  iIntros (Φ) "(#Hinit & H) HΦ". iNamed "H".
+  iApply wp_State__create_named_orphan_au.
+  iFrame "#". iFrame "%".
+  iFrame "Hdeepown_i Hown_reserved_frag".
+  iApply fupd_mask_intro.
+  { Timeout 10 set_solver. }
+  iIntros "Hmask".
+  iIntros (i' kobj' uid) "Hpost".
+  iMod "Hmask" as "_".
+  iModIntro. iNext.
+  iApply ("HΦ" $! i' kobj' uid with "Hpost").
+Qed.
+
+Lemma wp_State__PersistentVolumeClaimCreate_named_orphan
+    γ l namespace key pvc_l pvc :
+  {{{ is_pkg_init apimodel ∗
+      "#Hisk" ∷ is_kubernetes γ l ∗
+      "%Hvalid" ∷
+        ⌜ PersistentVolumeClaimV.valid_named_create namespace pvc ⌝ ∗
+      "%Hns_nonempty" ∷ ⌜ namespace ≠ ""%go ⌝ ∗
+      "%Hns_valid" ∷ ⌜ valid_namespace namespace ⌝ ∗
+      "%Hkey_eq" ∷ ⌜ key = {|
+        KKey.Kind' := PersistentVolumeClaimV.kind;
+        KKey.Name' :=
+          pvc.(PersistentVolumeClaimV.ObjectMeta').(ObjectMetaV.Name');
+        KKey.Namespace' := namespace
+      |} ⌝ ∗
+      "%Hparent_none" ∷
+        ⌜ obj_parent_ref (KObjectV.PersistentVolumeClaim pvc) = None ⌝ ∗
+      "Hdeepown_l" ∷ PersistentVolumeClaimV.deepown_l pvc_l pvc 1 ∗
+      "Hown_reserved_frag" ∷ own_reserved_frag γ key
+  }}}
+    l @! (go.PointerType apimodel.State) @!
+      "PersistentVolumeClaimCreate" #namespace #pvc_l
+  {{{ pvc_l' pvc' uid, RET (#pvc_l', #interface.nil);
+      "%Hvalid'" ∷
+        ⌜ KObjectV.valid (KObjectV.PersistentVolumeClaim pvc') ⌝ ∗
+      "%Hmeta_created" ∷
+        ⌜ ObjectMetaV.named_created namespace
+            pvc.(PersistentVolumeClaimV.ObjectMeta')
+            pvc'.(PersistentVolumeClaimV.ObjectMeta') ⌝ ∗
+      "%Hspec_created" ∷
+        ⌜ ObjectSpecV.created
+            (ObjectSpecV.PersistentVolumeClaimSpec
+              pvc.(PersistentVolumeClaimV.Spec'))
+            (ObjectSpecV.PersistentVolumeClaimSpec
+              pvc'.(PersistentVolumeClaimV.Spec')) ⌝ ∗
+      "%Hstatus_created" ∷
+        ⌜ ObjectStatusV.created
+            (ObjectStatusV.PersistentVolumeClaimStatus
+              pvc.(PersistentVolumeClaimV.Status'))
+            (ObjectStatusV.PersistentVolumeClaimStatus
+              pvc'.(PersistentVolumeClaimV.Status')) ⌝ ∗
+      "%Hkey_eq'" ∷ ⌜ key = PersistentVolumeClaimV.key pvc' ⌝ ∗
+      "%Huid_eq" ∷
+        ⌜ uid =
+          pvc'.(PersistentVolumeClaimV.ObjectMeta').(ObjectMetaV.UID') ⌝ ∗
+      "Hdeepown_l" ∷ PersistentVolumeClaimV.deepown_l pvc_l' pvc' 1 ∗
+      "Hown_meta_frag" ∷ own_meta_frag γ key uid 1
+        pvc'.(PersistentVolumeClaimV.ObjectMeta') ∗
+      "Hown_spec_frag" ∷ own_spec_frag γ key uid 1
+        (ObjectSpecV.PersistentVolumeClaimSpec
+          pvc'.(PersistentVolumeClaimV.Spec')) ∗
+      "Hown_status_frag" ∷ own_status_frag γ key uid 1
+        (ObjectStatusV.PersistentVolumeClaimStatus
+          pvc'.(PersistentVolumeClaimV.Status')) ∗
+      "Hown_children_frag" ∷ own_children_frag γ key uid 1 ∅
+  }}}.
+Proof.
+  iIntros (Φ) "(#Hinit & H) HΦ". iNamed "H".
+  wp_method_call.
+  rewrite /apimodel.State__PersistentVolumeClaimCreateⁱᵐᵖˡ.
+  wp_call. wp_auto.
+  iAssert (KObjectV.deepown_i
+      (interface.mk (go.PointerType v1.PersistentVolumeClaim) #pvc_l)
+      (KObjectV.PersistentVolumeClaim pvc) 1)
+    with "[Hdeepown_l]" as "Hdeepown_i".
+  { iExists pvc_l. iSplit; [done|]. iFrame. }
+  wp_apply (wp_State__create_named_orphan
+    γ l PersistentVolumeClaimV.kind namespace key
+    (interface.mk (go.PointerType v1.PersistentVolumeClaim) #pvc_l)
+    (KObjectV.PersistentVolumeClaim pvc)
+    with "[$Hinit $Hisk $Hdeepown_i $Hown_reserved_frag]").
+  { iPureIntro.
+    rewrite KObjectV.valid_named_create_eq_valid_named_create2 /=.
+    split_and!; done. }
+  iIntros (i' kobj' uid) "Hpost". iNamed "Hpost".
+  destruct kobj' as [pod'|rs'|pvc'|sts']; try done.
+  iDestruct "Hdeepown_i" as (pvc_l') "[%Hi' Hdeepown_l]".
+  wp_auto.
+  unfold KObjectV.valid_interface in Hi'. rewrite Hi'.
+  change (go.PointerType api_core_v1.PersistentVolumeClaim) with
+    (go.PointerType v1.PersistentVolumeClaim).
+  cbn [interface.ty interface.v].
+  replace
+    (if decide
+      (go.PointerType v1.PersistentVolumeClaim =
+       go.PointerType v1.PersistentVolumeClaim)
+     then #pvc_l' else #null)%V
+    with (#pvc_l')%V by (rewrite decide_True; done).
+  replace
+    (bool_decide
+      (go.PointerType v1.PersistentVolumeClaim =
+       go.PointerType v1.PersistentVolumeClaim))
+    with true by (symmetry; apply bool_decide_eq_true_2; done).
+  wp_auto.
+  iApply "HΦ". iFrame. iPureIntro. split_and!; done.
+Qed.
+
+End proof.
