src/proof/kubernetes_model/errors.v
@@ -1,5 +1,0 @@
-From New.proof Require Import prelude empty_ffi.
-
-Axiom conflict_error: interface.t → Prop.
-Axiom conflict_error_dec: ∀ err, Decision (conflict_error err).
-Global Existing Instance conflict_error_dec.
