src/proof/kubernetes_model/get_reserved.v
@@ -1,0 +1,95 @@
+From New.proof Require Import prelude empty_ffi.
+From New.proof.kubernetes_model Require Export get.
+
+Section proof.
+Context `{hG: !heapGS Σ} `{!ffi_semantics _ _}.
+Context {sem : go.Semantics} {package_sem : apimodel.Assumptions}.
+Context `{!kubernetesModelG Σ}.
+Local Set Default Proof Using "All".
+
+(* A reserved key is disjoint from the authoritative object map.  Therefore a
+   lookup at that key takes the model's concrete NotFound branch while
+   preserving the reservation for a subsequent create.  The AU exposes the
+   reservation only for the atomic model-state access. *)
+Lemma wp_State__get_reserved_au γ l key :
+  ∀ Φ,
+  ( is_pkg_init apimodel ∗
+    is_kubernetes γ l ∗
+    |={⊤,∅}=>
+      "Hown_reserved_frag" ∷ own_reserved_frag γ key ∗
+      "Hclose" ∷ (∀ err,
+        ⌜ not_found_error err ⌝ ∗
+        own_reserved_frag γ key
+          ={∅,⊤}=∗ ▷ Φ (#interface.nil, #err)%V)
+  ) -∗
+  WP l @! (go.PointerType apimodel.State) @! "get" #key {{ Φ }}.
+Proof.
+  iIntros (Φ) "(#Hpkg & #Hkinv & Hau)".
+  iNamed "Hkinv".
+  wp_method_call. rewrite /apimodel.State__getⁱᵐᵖˡ. wp_call.
+  wp_apply wp_with_defer as "%defer Hdefer".
+  simpl subst. wp_auto.
+  wp_apply wp_Mutex__Lock; [done|].
+  iIntros "[Hown_Mutex H]". iNamedPrefix "H" "Hinv_". wp_auto.
+  wp_apply (wp_map_lookup2_KKey (go.InterfaceType [])
+    with "[$Hinv_Hown_phys]").
+  iIntros "Hinv_Hown_phys". wp_auto.
+  iDestruct (big_sepM2_dom with "Hinv_Hphys_abs_rep") as %Hdom_eq.
+  destruct (bool_decide (is_Some (phys_state !! key))) eqn:Hdecide.
+  { apply bool_decide_eq_true in Hdecide.
+    assert (∃ i, phys_state !! key = Some i) as [i Hlookup_phys] by done.
+    assert (∃ kobj, abs_state !! key = Some kobj) as [kobj Hlookup_abs].
+    { apply elem_of_dom. rewrite <- Hdom_eq. apply elem_of_dom.
+      eexists. done. }
+    iApply fupd_wp.
+    iMod "Hau" as "H". iNamed "H".
+    iPoseProof (reserved_keys.frag_elem_of_auth key
+      with "[$Hinv_Hown_reserved] [$Hown_reserved_frag]")
+      as "%Hkey_reserved".
+    assert (abs_state !! key = None) as Hlookup_abs_none.
+    { apply not_elem_of_dom. Timeout 10 set_solver. }
+    rewrite Hlookup_abs in Hlookup_abs_none. done. }
+  apply bool_decide_eq_false in Hdecide.
+  assert (phys_state !! key = None) as Hlookup_phys.
+  { destruct (phys_state !! key) as [i|] eqn:Hlookup_phys; [|done].
+    exfalso. apply Hdecide. done. }
+  rewrite /is_Some Hlookup_phys. wp_auto.
+  wp_apply (wp_newNotFoundError with "[$Hpkg]").
+  iIntros (err) "(%Herr_non_nil & %Hnot_found)". wp_auto.
+  iApply fupd_wp.
+  iMod "Hau" as "H". iNamed "H".
+  iMod ("Hclose" $! err with "[$Hown_reserved_frag]") as "HΦ".
+  { done. }
+  iModIntro.
+  iCombineNamed "Hinv_*" as "H".
+  wp_apply (wp_Mutex__Unlock _ (kubernetes_inv γ l)
+    with "[$Hown_Mutex H]").
+  { iNamed "H". iFrame. iFrame "#". done. }
+  iApply "HΦ".
+Qed.
+
+Lemma wp_State__get_reserved γ l key :
+  {{{ is_pkg_init apimodel ∗
+      "#Hisk" ∷ is_kubernetes γ l ∗
+      "Hown_reserved_frag" ∷ own_reserved_frag γ key
+  }}}
+    l @! (go.PointerType apimodel.State) @! "get" #key
+  {{{ err, RET (#interface.nil, #err);
+      "%Hnot_found" ∷ ⌜ not_found_error err ⌝ ∗
+      "Hown_reserved_frag" ∷ own_reserved_frag γ key
+  }}}.
+Proof.
+  iIntros (Φ) "(#Hinit & #Hisk & Hown_reserved_frag) HΦ".
+  iApply wp_State__get_reserved_au.
+  iFrame "#".
+  iApply fupd_mask_intro.
+  { Timeout 10 set_solver. }
+  iIntros "Hmask".
+  iFrame "Hown_reserved_frag".
+  iIntros (err) "Hpost".
+  iMod "Hmask" as "_".
+  iModIntro. iNext.
+  iApply ("HΦ" $! err with "Hpost").
+Qed.
+
+End proof.
